a few things about done states and lots of things about the stack

DFS.v
@@ -19,6 +19,7 @@ Module DFS (O: UsualOrderedType)(M: FMapInterface.Sfun O) (S St: FSetInterface.S
 Module P := FMapFacts.WProperties_fun O M.
 Module F := P.F.
 Module P2 := FSetProperties.WProperties_fun O S.
+Module O2 := OrderedTypeFacts O.
 
 (*First, we define the types we will need*)
 Definition vertex := O.t.
@@ -81,11 +82,6 @@ Inductive dfs_step: state -> state -> Prop :=
       of the remaining vertices and start again*).
 
 (*A few state-related definitions to make the proofs simpler*)
-(*Is the DFS done? We will show that this condition holds iff there are no more steps*)
-Definition done' (s: state) : bool :=
-  match s with
-  | (_, _, _, _, _, start, finish, _) => S.is_empty start && S.is_empty finish
-  end.
 
 Definition get_time (s : state) : nat :=
   match s with
@@ -258,6 +254,11 @@ Proof.
   - apply valid_begins_with_start. assumption.
 Qed. 
 
+(** ** Results about discovery times **)
+(*In this section we prove several important results: namely that each vertex in the graph
+  is assigned a discovery time that is fixed, and that a vertex has a discovery time
+  iff it is no longer in remain_d*)
+
 (*If a vertex is discovered, it is not in remain_d*)
 Lemma discovered_vertex_not_remaining: forall s g o v,
   valid_dfs_state s g o ->
@@ -295,6 +296,7 @@ Proof.
         apply H1. auto.
 Qed.
 
+(*The add_to_stack function adds only vertices in the graph*)
 Lemma add_to_stack_adds_valid_vertices: forall v g r v' y,
   In (v', y) (add_to_stack v g r) ->
   G.contains_vertex g v' = true.
@@ -316,6 +318,7 @@ Definition get_graph (s: state) :=
   | (g, _, _, _, _, _, _, _) => g
   end.
 
+(*The graph does not change between states*)
 Lemma graph_is_constant: forall s g o,
   valid_dfs_state s g o ->
   get_graph s = g.
@@ -325,6 +328,7 @@ Proof.
   - inversion H0; subst; simpl in *; reflexivity.
 Qed.
 
+(*remain_d always contains only vertices in the graph g*)
 Lemma remain_d_contains_valid_vertices: forall s g o v,
   valid_dfs_state s g o ->
   S.mem v (get_remain_d s) = true ->
@@ -341,6 +345,7 @@ Proof.
       apply IHvalid_dfs_state. apply H1.
 Qed.
 
+(*Every vertex on the stack is in graph g*)
 Lemma stack_contains_valid_vertices: forall s g o v st (y: option vertex),
   valid_dfs_state s g o ->
   get_stack s = st ->
@@ -377,6 +382,7 @@ Proof.
       * destruct H1.
 Qed.
 
+(*If a vertex has a discovery time, it is in the graph*)
 Lemma discovered_vertices_in_graph: forall s g o v n,
   valid_dfs_state s g o ->
   M.find v (get_d_times s) = Some n ->
@@ -438,4 +444,456 @@ Proof.
   - apply IHmulti. eapply step. apply H. apply H1. eapply discovery_time_constant_step.
     apply H. apply H0. apply H1.
 Qed. 
+
+(** ** The done condition **)
+
+(*We are done if there are no more vertices to discover or finish*)
+Definition done (s: state) : bool :=
+  S.is_empty (get_remain_f s) && S.is_empty (get_remain_d s).
+
+(*Alternately, we are done if there are no more vertices to finish*)
+Definition done' (s: state) : bool :=
+  S.is_empty (get_remain_f s).
+
+(*If a vertex still has to be discovered, then it still has to be finished*)
+Lemma vertex_in_finish_if_not_discovered: forall s g o,
+  valid_dfs_state s g o ->
+  (forall x, 
+  S.mem x (get_remain_d s) = true ->
+  S.mem x (get_remain_f s) = true).
+Proof.
+  intros. induction H.
+  - unfold start_state in *; simpl in *. assumption.
+  - inversion H1; subst; simpl in *.
+    + apply IHvalid_dfs_state. apply S.mem_1. eapply S.remove_3.
+      apply S.mem_2. apply H0.
+    + assert (x <> x0). intro. subst. rewrite P2.FM.remove_b in H0. rewrite andb_true_iff in H0.
+      destruct H0. unfold P2.FM.eqb in H3. destruct (O.eq_dec x0 x0). inversion H3. apply n.
+      apply eq_refl. Search S.remove. rewrite P2.Dec.F.remove_neq_b in H0. apply IHvalid_dfs_state.
+      apply H0. auto.
+    + assert (x <> x0). intro. subst. rewrite H2 in H0. inversion H0. rewrite P2.Dec.F.remove_neq_b.
+      apply IHvalid_dfs_state. apply H0. auto.
+    + apply IHvalid_dfs_state. apply H0.
+    + apply IHvalid_dfs_state. apply H0.
+Qed. 
+
+(*A non empty set has at least one element*)
+Lemma non_empty_set_has_elements: forall (s: S.t),
+  (S.is_empty s) = false <-> exists x, S.In x s.
+Proof.
+  intros. split; intros.
+  - assert (~S.Empty s). intro. apply S.is_empty_1 in H0. rewrite H0 in H. inversion H.
+    assert (S.cardinal s <> 0). intro. apply P2.cardinal_inv_1 in H1. contradiction.
+    apply P2.cardinal_inv_2b in H1. destruct H1. exists x. apply i.
+  - destruct H. destruct (S.is_empty s) eqn : ?.
+    + apply S.is_empty_2 in Heqb. apply P2.empty_is_empty_1 in Heqb.
+      setoid_rewrite Heqb in H. apply P2.Dec.F.empty_iff in H. destruct H.
+    + reflexivity.
+Qed.
+
+(*When all vertices are finished, all vertices have been discovered*)
+Lemma finish_discover_before_finishing : forall (s: state) g o,
+  valid_dfs_state s g o ->
+  S.is_empty (get_remain_f s) = true ->
+  S.is_empty (get_remain_d s) = true.
+Proof.
+  intros. destruct (S.is_empty (get_remain_d s)) eqn : ?.
+  + reflexivity.
+  + rewrite non_empty_set_has_elements in Heqb. destruct Heqb.
+    apply S.mem_1 in H1. eapply vertex_in_finish_if_not_discovered in H1.
+    apply S.mem_2 in H1. apply S.is_empty_2 in H0. apply P2.empty_is_empty_1 in H0.
+    setoid_rewrite H0 in H1. apply P2.Dec.F.empty_iff in H1. destruct H1. apply H.
+Qed.
+
+Lemma done_done': forall s g o,
+  valid_dfs_state s g o ->
+  done s = done' s.
+Proof.
+  intros. unfold done. unfold done'. remember s as s'. destruct s. repeat(destruct p).
+  simpl. assert (t = get_remain_f s'). subst; simpl; reflexivity. rewrite Heqs'.
+  simpl. assert (t0 = get_remain_d s'). subst; simpl; reflexivity.
+  destruct (S.is_empty t) eqn : ?.
+  - apply finish_discover_before_finishing in H. rewrite <- H1 in H. rewrite H. reflexivity.
+    rewrite <- H0. apply Heqb.
+  - destruct (S.is_empty t0); reflexivity.
+Qed. 
+
+Lemma empty_set_no_elts: forall s x,
+  S.is_empty s = true /\ S.mem x s = true -> False.
+Proof.
+  intros. destruct H. apply S.is_empty_2 in H. apply P2.empty_is_empty_1 in H.
+      setoid_rewrite H in H0. rewrite P2.Dec.F.empty_b in H0. inversion H0.
+Qed.
+
+Ltac empty_set_mem :=
+  match goal with
+  | [H : S.is_empty ?s = true |- _] => 
+    match goal with
+    | [H1 : S.mem _ s = true |- _ ] =>
+      exfalso; eapply empty_set_no_elts; split;
+      try(apply H); try(apply H1)
+    end
+  end.
+
+Lemma add_to_stack_adds_parent: forall v g r x y,
+  In (x,y) (add_to_stack v g r) ->
+  y = Some v.
+Proof.
+  intros. unfold add_to_stack in H. destruct (G.neighbors_set g v).
+  assert (forall x y l, In (x,y)(fold_right (fun (v0 : S.elt) (t : list (S.elt * option O.t)) => if S.mem v0 r then (v0, Some v) :: t else t)
+         nil l) -> y = Some v). { intros. induction l; simpl in H0. destruct H0.
+        destruct (S.mem a r). simpl in H0. destruct H0. inversion H0. reflexivity. apply IHl.
+        apply H0. apply IHl. apply H0. }
+  eapply H0. apply H. inversion H.
+Qed.
+
+Lemma only_add_yet_to_be_discovered: forall v g r x y,
+  In (x,y) (add_to_stack v g r) ->
+  S.mem x r = true.
+Proof.
+  intros. unfold add_to_stack in H. destruct (G.neighbors_set g v).
+  assert (forall x y l, In (x, y)
+      (fold_right (fun (v0 : S.elt) (t : list (S.elt * option O.t)) => if S.mem v0 r then (v0, Some v) :: t else t)
+         nil l) -> S.mem x r = true). { intros. induction l; simpl in H0. destruct H0. destruct (S.mem a r) eqn : ?.
+        simpl in H0. destruct H0. inversion H0; subst. apply Heqb. all: apply IHl; apply H0. }
+  eapply H0. apply H. inversion H.
+Qed.
+
+Lemma only_add_neighbors: forall v g r x y,
+  In (x,y) (add_to_stack v g r) ->
+  G.contains_edge g v x = true.
+Proof.
+  intros. unfold add_to_stack in H. destruct (G.neighbors_set g v) eqn : ?.
+  - assert (forall x y l, In (x, y)
+      (fold_right (fun (v0 : S.elt) (t : list (S.elt * option O.t)) => if S.mem v0 r then (v0, Some v) :: t else t)
+         nil (l)) -> In x l). { intros. induction l; simpl in H0. destruct H0. destruct (S.mem a r). simpl in H0.
+      destruct H0. inversion H0; subst. simpl. left. reflexivity. simpl. right. apply IHl. apply H0.
+      simpl. right. apply IHl. apply H0. }
+    assert (In x (S.elements t)). eapply H0. apply H. clear H0. rewrite In_InA_equiv in H1.
+    apply S.elements_2 in H1. rewrite <- G.neighbors_set_2 in H1. apply H1. apply Heqo.
+    - inversion H.
+Qed.
+
+Lemma vertices_not_finished_on_stack: forall s g o v,
+  valid_dfs_state s g o ->
+  S.mem v (get_remain_d s) = false ->
+  S.mem v (get_remain_f s) = true ->
+  (exists y, In (v, y) (get_stack s)).
+Proof.
+  intros. generalize dependent v. induction H; intros; subst; simpl in *.
+  - rewrite H1 in H0. inversion H0.
+  - inversion H0; subst; simpl in *.
+    + destruct (O.eq_dec v x).
+      * setoid_rewrite e. exists None. apply in_or_app. right. simpl. left. reflexivity.
+      * rewrite P2.Dec.F.remove_neq_b in H1. apply IHvalid_dfs_state in H1. destruct H1.
+        exists x0. apply in_or_app. right. simpl. apply H1. apply H2. auto.
+    + destruct (O.eq_dec v x).
+      * setoid_rewrite e. exists (Some y). apply in_or_app. right. simpl. left. reflexivity.
+      * rewrite P2.Dec.F.remove_neq_b in H1. apply IHvalid_dfs_state in H1. destruct H1.
+        exists x0. apply in_or_app. right. simpl. apply H1. apply H2. auto.
+    + destruct (O.eq_dec v x).
+      * setoid_rewrite <- e in H2. rewrite P2.FM.remove_b in H2. rewrite andb_true_iff in H2.
+        destruct H2. unfold P2.FM.eqb in H5. destruct (O.eq_dec v v). inversion H5.
+        exfalso. apply n. apply eq_refl.
+      * rewrite P2.Dec.F.remove_neq_b in H2. apply IHvalid_dfs_state in H1. destruct H1.
+        destruct H1. inversion H1; subst. exfalso. apply n. apply eq_refl. exists x0. apply H1.
+        apply H2. auto.
+    + destruct (O.eq_dec x v).
+      * setoid_rewrite e in H4. rewrite H4 in H2. inversion H2.
+      * apply IHvalid_dfs_state in H1. destruct H1. destruct H1. inversion H1; subst.
+        exfalso. apply n. apply eq_refl. exists x0. apply H1. apply H2.
+    + apply IHvalid_dfs_state in H1. destruct H1. destruct H1. apply H2.
+Qed.
+
+Fixpoint list_neq (l1 l2: list O.t) :=
+  match l1, l2 with
+  | x1 :: t1, x2 :: t2 => if O.eq_dec x1 x2 then list_neq t1 t2 else true
+  | nil, nil => false
+  | _, _ => true
+  end.
+
+Lemma list_eq_neq: forall l1 l2,
+  l1 <> l2 <-> list_neq l1 l2 = true.
+Proof.
+  intros. split; intros.
+  - generalize dependent l2. induction l1; intros.
+    + simpl. destruct l2. contradiction. reflexivity.
+    + simpl. destruct l2 eqn : ?. reflexivity.
+      destruct (O.eq_dec a t).
+      * setoid_rewrite e in H. assert (l1 <> l). intro. subst. contradiction.
+        apply IHl1. apply H0.
+      * reflexivity.
+  - intro. subst. induction l2. simpl in H. inversion H. simpl in H.
+    destruct (O.eq_dec a a). apply IHl2. apply H. apply n. apply eq_refl.
+Qed. 
+
+Lemma list_neq_has_diff_elements: forall (l1 l2: list O.t),
+  StronglySorted O.lt l1 ->
+  StronglySorted O.lt l2 ->
+  l1 <> l2 ->
+  (exists x, In x l1 /\ ~In x l2) \/ (exists x, ~In x l1 /\ In x l2).
+Proof.
+  intros. rewrite list_eq_neq in H1. generalize dependent l2; induction l1; intros.
+  - simpl in H1. destruct l2 eqn : ?. inversion H1. right. exists t.
+    split. auto. simpl. left. reflexivity.
+  - simpl in H1. destruct l2 eqn : ?.
+    + left. exists a. split. simpl. left. reflexivity. auto.
+    + inversion H0; subst. inversion H; subst. destruct (O.eq_dec a t) eqn : ?. 
+      * setoid_rewrite e. apply IHl1 in H4. destruct H4.
+        -- destruct H2. destruct H2. assert (O.lt t x). rewrite Forall_forall in H7.
+           setoid_rewrite <- e. eapply H7. apply H2. left. exists x. split. simpl.
+           right. apply H2. simpl. intro. destruct H8. subst. apply O.lt_not_eq in H4.
+           apply H4. apply eq_refl. contradiction.
+        -- destruct H2. destruct H2. assert (O.lt t x). rewrite Forall_forall in H5.
+           eapply H5. apply H3. right. exists x. split.  simpl. intro. destruct H8.
+           subst. apply O.lt_not_eq in H4. apply H4. apply eq_refl. contradiction.
+           simpl. right. apply H3.
+        -- apply H6.
+        -- apply H1.
+      * pose proof (O2.lt_total a t). destruct H2.
+        -- left. exists a. split. simpl. left. reflexivity. rewrite Forall_forall in H5.
+           simpl. intro. destruct H3. subst. apply n. apply eq_refl. apply H5 in H3.
+           apply O2.lt_le in H3. contradiction.
+        -- destruct H2.
+            ** subst. exfalso. apply n. apply eq_refl.
+            ** right. exists t. split. simpl. intro. destruct H3. subst. apply n. apply eq_refl.
+               rewrite Forall_forall in H7. apply H7 in H3. apply O2.lt_le in H3.
+               contradiction. simpl. left. reflexivity.
+Qed. 
+
+Lemma unequal_sets: forall s1 s2,
+  S.equal s1 s2 = false ->
+  (exists v, S.In v s1 /\ ~S.In v s2) \/ (exists v, ~S.In v s1 /\ S.In v s2).
+Proof.
+  intros. destruct (list_neq (S.elements s1) (S.elements s2)) eqn : ?.
+  - rewrite <- list_eq_neq in Heqb. apply list_neq_has_diff_elements in Heqb.
+    destruct Heqb.
+    + destruct H0. destruct H0. rewrite In_InA_equiv in *. apply S.elements_2 in H0.
+      assert (~S.In x s2). intro. apply S.elements_1 in H2. contradiction.
+      left. exists x. split; assumption.
+    + destruct H0. destruct H0. rewrite In_InA_equiv in *. apply S.elements_2 in H1.
+      assert (~S.In x s1). intro. apply S.elements_1 in H2. contradiction.
+      right. exists x. split; assumption.
+    + apply Sorted_StronglySorted. unfold Relations_1.Transitive. intros.
+      eapply O.lt_trans. apply H0. apply H1. apply S.elements_3.
+    + apply Sorted_StronglySorted. unfold Relations_1.Transitive. intros.
+      eapply O.lt_trans. apply H0. apply H1. apply S.elements_3.
+  - destruct (list_eq_dec O.eq_dec (S.elements s1) (S.elements s2)).
+    + assert (forall x, S.In x s1 <-> S.In x s2). { intros.
+      split; intros; apply S.elements_1 in H0.  all: apply S.elements_2.
+      rewrite <- e. assumption. rewrite e. assumption. }
+      assert (~S.Equal s1 s2). intro. apply S.equal_1 in H1. rewrite H1 in H. inversion H.
+      assert (S.Equal s1 s2). unfold S.Equal. apply H0. contradiction.
+    + rewrite list_eq_neq in n. rewrite n in Heqb. inversion Heqb.
+Qed.
+
+(*When stack is empty, same vertices left to be discovered and finished*)
+Lemma empty_stack_no_gray: forall s g o,
+  valid_dfs_state s g o ->
+  get_stack s = nil ->
+  S.Equal (get_remain_d s) (get_remain_f s).
+Proof.
+(*Idea: either the two sets are equal or not. If not, then there is one element in 1 that is not in another*)
+(*This element cannot be in remain_f, since then it would have to be in remain_d. So there is an
+  element in remain_d not in remain_f, by previous result, stack is nonempty, a contradiction*)
+intros. apply S.equal_2. destruct (S.equal (get_remain_d s) (get_remain_f s)) eqn : ?.
+ - reflexivity.
+ - apply unequal_sets in Heqb. destruct Heqb.
+  + destruct H1. destruct H1. apply P2.FM.mem_iff in H1. 
+    destruct (S.mem x (get_remain_f s)) eqn : ?. apply P2.FM.mem_iff in Heqb.
+    contradiction. eapply vertex_in_finish_if_not_discovered in H1. rewrite Heqb in H1.
+    inversion H1. apply H.
+  + destruct H1. destruct H1.  apply P2.FM.mem_iff in H2. destruct (S.mem x (get_remain_d s)) eqn : ?.
+    apply P2.FM.mem_iff in Heqb. contradiction. eapply vertices_not_finished_on_stack in Heqb.
+    rewrite H0 in Heqb. destruct Heqb. simpl in H3. destruct H3. apply H. apply H2.
+Qed.
+
+(*This gives us an idea that our choice of the [done] property was a good one: a state is done
+  if it cannot step, actually might be better to do existence way first but well see*)
+Lemma done_cannot_step: forall s g o,
+  valid_dfs_state s g o ->
+  (done' s = true <-> (forall s', ~dfs_step s s')).
+Proof.
+  intros. split; intros.
+  - intro contra. inversion contra; unfold done' in *; subst; simpl in *.
+    + remember (g0, f, f_times, d_times, time, remain_d, remain_f, (x, None) :: tl) as s.
+      assert (S.is_empty (get_remain_f s) = true) by (subst; simpl; assumption).
+      eapply finish_discover_before_finishing in H2. subst; simpl in *.
+      empty_set_mem. apply H.
+    + remember (g0, t :: f, f_times, d_times, time, remain_d, remain_f, (x, Some y) :: tl) as s.
+      assert (S.is_empty (get_remain_f s) = true) by (subst; simpl; assumption).
+      eapply finish_discover_before_finishing in H2. subst; simpl in *.
+      empty_set_mem. apply H.
+    + empty_set_mem.
+    + rewrite andb_false_iff in H3. destruct H3. 
+      * remember (g0, f, f_times, d_times, time, remain_d, remain_f, (x, y) :: tl) as s.
+        assert (S.is_empty (get_remain_f s) = true) by (subst; simpl; assumption).
+        eapply finish_discover_before_finishing in H4. subst; simpl in *.
+        rewrite H4 in H3. inversion H3. apply H.
+      * rewrite H3 in H0. inversion H0.
+    + remember (g0, f, f_times, d_times, time, remain_d, remain_f, nil) as s.
+      assert (S.is_empty (get_remain_f s) = true) by (subst; simpl in *; assumption).
+      eapply finish_discover_before_finishing in H2. subst; simpl in *.
+      apply S.min_elt_1 in H1. apply S.mem_1 in H1. empty_set_mem. apply H.
+  - induction H; subst; unfold done'; simpl in *.
+    + destruct (S.is_empty (G.set_of_graph g)) eqn : ?.
+      * reflexivity.
+      * unfold start_state in H0. destruct o.
+        -- destruct (G.contains_vertex g v) eqn : ?.
+          ++ exfalso. eapply H0. apply dfs_discover_root. apply S.mem_1.
+             rewrite <- G.set_of_graph_1. apply Heqb0.
+          ++ destruct (S.min_elt (G.set_of_graph g)) eqn : ?.
+              ** exfalso. eapply H0. apply dfs_new_cc. apply Heqo.
+              ** apply S.min_elt_3 in Heqo. apply S.is_empty_1 in Heqo.
+                 rewrite Heqo in Heqb. inversion Heqb.
+       -- destruct (S.min_elt (G.set_of_graph g)) eqn : ?.
+          ++ exfalso. eapply H0. apply dfs_new_cc. apply Heqo.
+          ++ apply S.min_elt_3 in Heqo. apply S.is_empty_1 in Heqo.
+             rewrite Heqo in Heqb. inversion Heqb.
+    + inversion H1; subst; simpl in *.
+      * destruct ( add_to_stack x g0 remain_d) eqn : ?.
+        -- exfalso. eapply H0. simpl. apply dfs_finish. rewrite P2.FM.remove_b. rewrite andb_false_iff.
+           right. unfold P2.FM.eqb. destruct (O.eq_dec x x). reflexivity. exfalso.
+            apply n. apply eq_refl. 
+           remember (g0, f, f_times, d_times, time, remain_d, remain_f, (x, None) :: tl)  as s.
+           assert (S.mem x (get_remain_d s) = true) by (subst; simpl; assumption).
+           eapply vertex_in_finish_if_not_discovered in H3. subst; simpl in *. apply H3.
+           apply H.
+        -- exfalso. destruct p. assert (o0 = Some x). { eapply add_to_stack_adds_parent. 
+            rewrite Heqs. simpl. left. reflexivity. } eapply H0. rewrite H3. apply dfs_discover_child.
+            assert (G.contains_edge g x t = true). eapply only_add_neighbors.
+            assert (g = g0). remember (g0, f, f_times, d_times, time, remain_d, remain_f, (x, None) :: tl) as s'. 
+            assert (g0 = get_graph s') by (subst; simpl; reflexivity). rewrite H4. symmetry. eapply graph_is_constant.
+            apply H. rewrite H4. simpl. rewrite Heqs. simpl. left. reflexivity. 
+            apply G.contains_edge_3 in H4. rewrite P2.FM.remove_neq_b. eapply only_add_yet_to_be_discovered.
+            rewrite Heqs. simpl. left. reflexivity. apply H4.
+      * destruct ( add_to_stack x g0 remain_d) eqn : ?.
+        -- exfalso. eapply H0. simpl. apply dfs_finish. rewrite P2.FM.remove_b. rewrite andb_false_iff.
+           right. unfold P2.FM.eqb. destruct (O.eq_dec x x). reflexivity. exfalso.
+            apply n. apply eq_refl. 
+           remember (g0, t :: f, f_times, d_times, time, remain_d, remain_f, (x, Some y) :: tl)  as s.
+           assert (S.mem x (get_remain_d s) = true) by (subst; simpl; assumption).
+           eapply vertex_in_finish_if_not_discovered in H3. subst; simpl in *. apply H3.
+           apply H.
+        -- exfalso. destruct p. assert (o0 = Some x). { eapply add_to_stack_adds_parent. 
+            rewrite Heqs. simpl. left. reflexivity. } eapply H0. rewrite H3. apply dfs_discover_child.
+            assert (G.contains_edge g x t0 = true). eapply only_add_neighbors.
+            assert (g = g0). remember (g0, t :: f, f_times, d_times, time, remain_d, remain_f, (x, Some y) :: tl) as s'. 
+            assert (g0 = get_graph s') by (subst; simpl; reflexivity). rewrite H4. symmetry. eapply graph_is_constant.
+            apply H. rewrite H4. simpl. rewrite Heqs. simpl. left. reflexivity. 
+            apply G.contains_edge_3 in H4. rewrite P2.FM.remove_neq_b. eapply only_add_yet_to_be_discovered.
+            rewrite Heqs. simpl. left. reflexivity. apply H4.
+       * destruct (S.is_empty (S.remove x remain_f)) eqn : ?. 
+         -- reflexivity.
+         -- destruct tl. destruct (S.min_elt (S.remove x remain_f)) eqn : ?.
+            ++ assert (A:=Heqo1). apply S.min_elt_1 in Heqo1. apply S.mem_1 in Heqo1.
+               destruct (S.mem e remain_d) eqn : ?.
+               ** exfalso. 
+                   remember ((g0, f, M.add x time f_times, d_times, time + 1, remain_d, S.remove x remain_f, nil)) as s'.
+ assert (S.Equal (get_remain_d s') (get_remain_f s')). { eapply empty_stack_no_gray.
+      eapply step. apply H. apply H1. subst. reflexivity. } subst; simpl in H4. 
+    (*Figure this out tomorrow*)
+      setoid_rewrite <- H4 in A.
+               ** (S.remove x remain_f)). {
+                  
+                  eapply empty_stack_no_gray.
+
+
+ Search S.min_elt. rewrite non_empty_set_has_elements in Heqb. destruct Heqb.
+            apply S.mem_1 in H4. destruct (S.mem x0 (remain_d)) eqn : ?.
+            ++ 
+        +
+
+
+
+(*finish case, we could be done, or if there is still someone in remain_f, we have to prove that
+           they are still on the stack - for tomorrow*)
+           
+            
+            
+
+ 
+        -- unfold start_state in H0.
+           dest rewrite non_empty_set_has_elements in Heqb. Search S.min_elt.
+        d
+
+ auto.  empty_set_mem.
+      apply S.is_empty_2 in H2. apply P2.empty_is_empty_1 in H2.
+      setoid_rewrite H2 in H1. rewrite P2.Dec.F.empty_b in H1. inversion H1. apply H.
+    + 
+  
+
+
+
+  induction H; unfold done' in *; subst; simpl in *.
+  - intro contra. unfold start_state in contra. destruct o.
+    destruct (G.contains_vertex g v) eqn : ?.
+    + rewrite G.set_of_graph_1 in Heqb. apply S.is_empty_2 in H0.
+        apply P2.empty_is_empty_1 in H0. setoid_rewrite H0 in Heqb.
+        rewrite P2.FM.empty_iff in Heqb. destruct Heqb.
+    + inversion contra; subst; simpl in *.
+      * apply S.min_elt_1 in H8.  apply S.is_empty_2 in H0.
+        apply P2.empty_is_empty_1 in H0. setoid_rewrite H0 in H8.
+        rewrite P2.FM.empty_iff in H8. apply H8.
+    + inversion contra; subst; simpl in *. apply S.min_elt_1 in H8.  apply S.is_empty_2 in H0.
+        apply P2.empty_is_empty_1 in H0. setoid_rewrite H0 in H8.
+        rewrite P2.FM.empty_iff in H8. apply H8.
+  - intro contra. inversion H1; subst; simpl in *.
+    + remember ((g0, f, f_times, d_times, time, remain_d, remain_f, (x, None) :: tl)) as s.
+      assert (S.is_empty (get_remain_f s) = true). subst; simpl; assumption.
+      eapply finish_discover_before_finishing in H3. subst; simpl in *.
+      apply S.is_empty_2 in H3. apply P2.empty_is_empty_1 in H3.
+      setoid_rewrite H3 in H2. rewrite P2.FM.empty_b in H2. inversion H2. apply H.
+    + remember ((g0, t ::f, f_times, d_times, time, remain_d, remain_f, (x, Some y) :: tl)) as s.
+      assert (S.is_empty (get_remain_f s) = true). subst; simpl; assumption.
+      eapply finish_discover_before_finishing in H3. subst; simpl in *.
+      apply S.is_empty_2 in H3. apply P2.empty_is_empty_1 in H3.
+      setoid_rewrite H3 in H2. rewrite P2.FM.empty_b in H2. inversion H2.  apply H.
+    +  
+
+
+ rewri simpl. simpl in *. inversion contra; subst; simpl in *.
+    + destruct o. destruct (G.contains_vertex g v) eqn : ?.
+      * rewrite G.set_of_graph_1 in Heqb. apply S.is_empty_2 in H0.
+        apply P2.empty_is_empty_1 in H0. setoid_rewrite H0 in Heqb.
+        rewrite P2.FM.empty_iff in Heqb. destruct Heqb.
+      * inversion H8.
+      * inversion H8.
+    + 
+    +
+
+
+Lemma done_cannot_step: forall s g,
+  valid_dfs_state s g ->
+  done' s = true ->
+  (forall s', ~dfs_step s s').
+Proof.
+  intros. intro. unfold done' in H0. inversion H1; subst; simpl in *.
+  - remember ((g0, t, f_times, d_times, time, remain_d, remain_f, (x, y) :: tl)) as s.
+    assert (remain_f_of_state s = remain_f). subst; simpl; reflexivity.
+    rewrite <- H3 in H0. apply (finish_discover_before_finishing s g H) in H0.
+    apply S.is_empty_2 in H0. apply P2.empty_is_empty_1 in H0.
+    assert (remain_d_of_state s = remain_d). subst; simpl; reflexivity. 
+    rewrite H4 in H0. setoid_rewrite H0 in H2. apply S.mem_2 in H2. apply P2.FM.empty_iff in H2.
+    apply H2.
+  - apply S.mem_2 in H3. apply S.is_empty_2 in H0. apply P2.empty_is_empty_1 in H0.
+    setoid_rewrite H0 in H3. apply P2.FM.empty_iff in H3. apply H3.
+  - apply S.mem_2 in H3. apply S.is_empty_2 in H0. apply P2.empty_is_empty_1 in H0.
+    setoid_rewrite H0 in H3. apply P2.FM.empty_iff in H3. apply H3.
+  - assert (S.is_empty remain_d = false). destruct (S.is_empty remain_d) eqn : ?.
+    apply S.is_empty_2 in Heqb. apply S.min_elt_1 in H2. apply P2.empty_is_empty_1 in Heqb.
+    setoid_rewrite Heqb in H2. apply P2.FM.empty_iff in H2. destruct H2. reflexivity.
+    remember (g0, t, f_times, d_times, time, remain_d, remain_f, []) as s.
+    assert (remain_f_of_state  s = remain_f). subst; simpl; reflexivity.
+    assert (remain_d_of_state s = remain_d). subst; reflexivity.
+    rewrite <- H4 in H0. eapply finish_discover_before_finishing in H0.
+    rewrite H5 in H0. rewrite H3 in H0. inversion H0. apply H.
+Qed. 
+
+
+
+Lemma all_vertices_discovered_at_end: forall s g o v,
+  valid_dfs_state s g o ->
+  done s ->
+  (exists n, M.find v (get_d_times s) = Some n).
 
